Drop the IO.fsti interface. Defining EStringEq

rupicola/io/IO.fst
@@ -1,98 +1,155 @@
 module IO
 
-(** we only have bools in STLC right now **)
-open Trace
-
 open FStar.Tactics.V1
 
-let theta = theta_unf
+include BaseTypes
+include Hist
+open Trace
 
-let unfold_theta #a :
-  Lemma (theta #a == theta_unf #a)
-  by (norm [delta_only [`%theta]])
-= ()
+noeq
+type io (a:Type u#a) : Type u#a =
+| Call : o:io_ops -> args:io_args o -> (io_res o args -> io a) -> io a
+| Return : a -> io a
 
+let io_return (#a:Type) (x:a) : io a =
+  Return x
+
+let rec io_bind
+  (#a:Type u#a)
+  (#b:Type u#b)
+  (l : io a)
+  (k : a -> io b) :
+  io b =
+  match l with
+  | Return x -> k x
+  | Call o args fnc ->
+      Call o args (fun i ->
+        io_bind #a #b (fnc i) k)
+
+let openfile (fnm:string) : io (resexn file_descr) =
+  Call OOpen fnm Return
+
+let read (fd:file_descr) : io (resexn string) =
+  Call ORead fd Return
+
+let write (x:file_descr * string) : io (resexn unit) =
+  Call OWrite x Return
+
+let close (fd:file_descr) : io (resexn unit) =
+  Call OClose fd Return
+
+let return = io_return
+let (let!@) = io_bind
+
+let op_wp (o:io_ops) (args:io_args o) : hist (io_res o args) =
+  to_hist
+    (fun h -> io_pre h o args)
+    (fun h res lt -> io_post h o args res /\ lt == [op_to_ev o args res])
+
+let rec theta #a (m:io a) : hist a =
+  match m with
+  | Return x -> hist_return x
+  | Call o args k -> hist_bind (op_wp o args) (fun r -> theta (k r))
+
+val theta_monad_morphism_ret (x:'a) :
+  Lemma (theta (return x) == hist_return x)
 let theta_monad_morphism_ret x =
   assert (theta (return x) == hist_return x) by (FStar.Tactics.compute ())
 
-val theta_monad_morphism_bind_ (m:io 'a) (k:'a -> io 'b) :
-  Lemma (theta_unf (io_bind m k) `hist_equiv` hist_bind (theta_unf m) (fun x -> theta_unf (k x)))
-let rec theta_monad_morphism_bind_ m k =
+val theta_monad_morphism_bind (m:io 'a) (k:'a -> io 'b) :
+  Lemma (theta (io_bind m k) `hist_equiv` hist_bind (theta m) (fun x -> theta (k x)))
+let rec theta_monad_morphism_bind m k =
   match m with
   | Return _ -> ()
   | Call o arg m' ->
     calc (hist_equiv) {
-      theta_unf (io_bind (Call o arg m') k);
+      theta (io_bind (Call o arg m') k);
       `hist_equiv` { _ by (compute ()) }
-      theta_unf (Call o arg (fun x -> io_bind (m' x) k));
-      `hist_equiv` { _ by (norm [delta_once [`%theta_unf]; iota]) }
-      hist_bind (op_wp o arg) (fun r -> theta_unf (io_bind (m' r) k));
+      theta (Call o arg (fun x -> io_bind (m' x) k));
+      `hist_equiv` { _ by (norm [delta_once [`%theta]; iota]) }
+      hist_bind (op_wp o arg) (fun r -> theta (io_bind (m' r) k));
       `hist_equiv` {
-        introduce forall r. theta_unf (io_bind (m' r) k) `hist_equiv` hist_bind (theta_unf (m' r)) (fun x -> theta_unf (k x)) with begin
-          theta_monad_morphism_bind_ (m' r) k
+        introduce forall r. theta (io_bind (m' r) k) `hist_equiv` hist_bind (theta (m' r)) (fun x -> theta (k x)) with begin
+          theta_monad_morphism_bind (m' r) k
         end;
-        lem_hist_bind_equiv (op_wp o arg) (op_wp o arg) (fun r -> theta_unf (io_bind (m' r) k)) (fun r -> hist_bind (theta_unf (m' r)) (fun x -> theta_unf (k x)))
+        lem_hist_bind_equiv (op_wp o arg) (op_wp o arg) (fun r -> theta (io_bind (m' r) k)) (fun r -> hist_bind (theta (m' r)) (fun x -> theta (k x)))
        }
-      hist_bind (op_wp o arg) (fun r -> hist_bind (theta_unf (m' r)) (fun x -> theta_unf (k x)));
-      `hist_equiv` { lemma_hist_bind_associativity (op_wp o arg) (fun r -> theta_unf (m' r)) (fun x -> theta_unf (k x)) }
-      hist_bind (hist_bind (op_wp o arg) (fun r -> theta_unf (m' r))) (fun x -> theta_unf (k x));
+      hist_bind (op_wp o arg) (fun r -> hist_bind (theta (m' r)) (fun x -> theta (k x)));
+      `hist_equiv` { lemma_hist_bind_associativity (op_wp o arg) (fun r -> theta (m' r)) (fun x -> theta (k x)) }
+      hist_bind (hist_bind (op_wp o arg) (fun r -> theta (m' r))) (fun x -> theta (k x));
       `hist_equiv` {
         assert (hist_equiv
-          (hist_bind (theta_unf (Call o arg m')) (fun x -> theta_unf (k x)))
-          (hist_bind (hist_bind (op_wp o arg) (fun r -> theta_unf (m' r))) (fun x -> theta_unf (k x)))
-        ) by (norm [delta_once [`%theta_unf]; zeta; iota];
+          (hist_bind (theta (Call o arg m')) (fun x -> theta (k x)))
+          (hist_bind (hist_bind (op_wp o arg) (fun r -> theta (m' r))) (fun x -> theta (k x)))
+        ) by (norm [delta_once [`%theta]; zeta; iota];
           apply_lemma (`lem_hist_equiv_reflexive)) }
-      hist_bind (theta_unf (Call o arg m')) (fun x -> theta_unf (k x));
+      hist_bind (theta (Call o arg m')) (fun x -> theta (k x));
     }
 
-let theta_monad_morphism_bind #a m k =
-  unfold_theta #a ;
-  theta_monad_morphism_bind_ m k
-
-val io_bind_equivalence_ #a #b (k k':a -> io b) (m:io a) :
+val io_bind_equivalence #a #b (k k':a -> io b) (m:io a) :
   Lemma (requires forall x. k x == k' x)
-        (ensures theta_unf (io_bind m k) `hist_equiv` theta_unf (io_bind m k'))
-let io_bind_equivalence_ (#a #b:Type) (k k':a -> io b) (m:io a) :
-  Lemma (requires forall x. k x == k' x)
-        (ensures theta_unf (io_bind m k) `hist_equiv` theta_unf (io_bind m k')) =
-  match m with
-  | Return _ -> ()
-  | Call o arg m' ->
-    calc (hist_equiv) {
-      theta_unf (io_bind (Call o arg m') k);
-      `hist_equiv` { theta_monad_morphism_bind_ (Call o arg m') k }
-      hist_bind (theta_unf (Call o arg m')) (fun x -> theta_unf (k x));
-      `hist_equiv` { _ by (norm [delta_once [`%theta_unf]; zeta;iota]) }
-      hist_bind (hist_bind (op_wp o arg) (fun r -> theta_unf (m' r))) (fun x -> theta_unf (k x));
-      `hist_equiv` { lemma_hist_bind_associativity (op_wp o arg) (fun r -> theta_unf (m' r)) (fun x -> theta_unf (k x)) }
-      hist_bind (op_wp o arg) (fun r -> hist_bind (theta_unf (m' r)) (fun x -> theta_unf (k x)));
-      `hist_equiv` {
-        lem_hist_bind_equiv (op_wp o arg) (op_wp o arg) (fun r -> hist_bind (theta_unf (m' r)) (fun x -> theta_unf (k x))) (fun r -> hist_bind (theta_unf (m' r)) (fun x -> theta_unf (k' x)))
-      }
-      hist_bind (op_wp o arg) (fun r -> hist_bind (theta_unf (m' r)) (fun x -> theta_unf (k' x)));
-      `hist_equiv` { lemma_hist_bind_associativity (op_wp o arg) (fun r -> theta_unf (m' r)) (fun x -> theta_unf (k' x)) }
-      hist_bind (hist_bind (op_wp o arg) (fun r -> theta_unf (m' r))) (fun x -> theta_unf (k' x));
-      `hist_equiv` {
-        assert (hist_equiv
-          (hist_bind (theta_unf (Call o arg m')) (fun x -> theta_unf (k' x)))
-          (hist_bind (hist_bind (op_wp o arg) (fun r -> theta_unf (m' r))) (fun x -> theta_unf (k' x)))
-        ) by (norm [delta_once [`%theta_unf]; zeta; iota];
-          apply_lemma (`lem_hist_equiv_reflexive))
-       }
-      hist_bind (theta_unf (Call o arg m')) (fun x -> theta_unf (k' x));
-      `hist_equiv` { theta_monad_morphism_bind_ m k' }
-      theta_unf (io_bind (Call o arg m') k');
-    }
-
+        (ensures theta (io_bind m k) `hist_equiv` theta (io_bind m k'))
 let io_bind_equivalence (#a #b:Type) (k k':a -> io b) (m:io a) :
   Lemma (requires forall x. k x == k' x)
         (ensures theta (io_bind m k) `hist_equiv` theta (io_bind m k')) =
-  unfold_theta #a ;
-  io_bind_equivalence_ k k' m
+  match m with
+  | Return _ -> ()
+  | Call o arg m' ->
+    calc (hist_equiv) {
+      theta (io_bind (Call o arg m') k);
+      `hist_equiv` { theta_monad_morphism_bind (Call o arg m') k }
+      hist_bind (theta (Call o arg m')) (fun x -> theta (k x));
+      `hist_equiv` { _ by (norm [delta_once [`%theta]; zeta;iota]) }
+      hist_bind (hist_bind (op_wp o arg) (fun r -> theta (m' r))) (fun x -> theta (k x));
+      `hist_equiv` { lemma_hist_bind_associativity (op_wp o arg) (fun r -> theta (m' r)) (fun x -> theta (k x)) }
+      hist_bind (op_wp o arg) (fun r -> hist_bind (theta (m' r)) (fun x -> theta (k x)));
+      `hist_equiv` {
+        lem_hist_bind_equiv (op_wp o arg) (op_wp o arg) (fun r -> hist_bind (theta (m' r)) (fun x -> theta (k x))) (fun r -> hist_bind (theta (m' r)) (fun x -> theta (k' x)))
+      }
+      hist_bind (op_wp o arg) (fun r -> hist_bind (theta (m' r)) (fun x -> theta (k' x)));
+      `hist_equiv` { lemma_hist_bind_associativity (op_wp o arg) (fun r -> theta (m' r)) (fun x -> theta (k' x)) }
+      hist_bind (hist_bind (op_wp o arg) (fun r -> theta (m' r))) (fun x -> theta (k' x));
+      `hist_equiv` {
+        assert (hist_equiv
+          (hist_bind (theta (Call o arg m')) (fun x -> theta (k' x)))
+          (hist_bind (hist_bind (op_wp o arg) (fun r -> theta (m' r))) (fun x -> theta (k' x)))
+        ) by (norm [delta_once [`%theta]; zeta; iota];
+          apply_lemma (`lem_hist_equiv_reflexive))
+       }
+      hist_bind (theta (Call o arg m')) (fun x -> theta (k' x));
+      `hist_equiv` { theta_monad_morphism_bind m k' }
+      theta (io_bind (Call o arg m') k');
+    }
 
+let thetaP m = wp2p (theta m)
+
+val wp2p_theta_bind (m:io 'a) (k:'a -> io 'b) :
+  Lemma (forall h.
+         wp2p (hist_bind (theta m) (fun x -> theta (k x))) h (** Kind of ugly. Can we use hist_post_bind? **)
+         `hist_post_equiv`
+         thetaP (io_bind m k) h)
 let wp2p_theta_bind m k =
   theta_monad_morphism_bind m k
 
+(** Trying to connect with hist_post_bind. Does not look like it holds.
+let lem_thetaP_bind #a #b (m:io a) (k:a -> io b) :
+  Lemma (forall h.
+         wp2p (hist_bind (theta m) (fun x -> theta (k x))) h
+        `hist_post_equiv`
+         hist_post_bind (thetaP m h) (fun lt r -> thetaP (k r) (h++lt))) =
+  assert (forall h.
+         wp2p (hist_bind (theta m) (fun x -> theta (k x))) h
+        `hist_post_equiv`
+         hist_post_bind (thetaP m h) (fun lt r -> thetaP (k r) (h++lt))) by (
+         norm [delta_only [`%hist_post_bind; `%thetaP; `%hist_bind; `%wp2p;
+         `%hist_post_bind'; `%hist_post_shift;`%hist_post_equiv;`%hist_post_ord]; iota];
+         let h = forall_intro () in
+         split ();
+         dump "H")
+**)
+val lem_theta_open (arg:io_args OOpen) (res:io_res OOpen arg) (h:history) :
+  Lemma (requires Inl? res ==> Inl?.v res == fresh_fd h)
+        (ensures thetaP (openfile arg) h (ev_lt (EvOpen arg res)) res)
 let lem_theta_open arg res h =
   introduce forall (p:hist_post h (io_res OOpen arg)). (theta (openfile arg)) h p ==> p (ev_lt (EvOpen arg res)) res with begin
     introduce _ ==> _ with _. begin
@@ -105,6 +162,25 @@ let lem_theta_open arg res h =
     end
   end
 
+val lem_theta_read (arg:io_args ORead) (res:io_res ORead arg) (h:history) :
+  Lemma (thetaP (read arg) h (ev_lt (EvRead arg res)) res)
+let lem_theta_read arg res h =
+  assert (thetaP (read arg) h (ev_lt (EvRead arg res)) res) by (compute ())
+
+val lem_theta_write (arg:io_args OWrite) (res:io_res OWrite arg) (h:history) :
+  Lemma (thetaP (write arg) h (ev_lt (EvWrite arg res)) res)
+let lem_theta_write arg res h =
+  assert (thetaP (write arg) h (ev_lt (EvWrite arg res)) res) by (compute ())
+
+val lem_theta_close (arg:io_args OClose) (res:io_res OClose arg) (h:history) :
+  Lemma (thetaP (close arg) h (ev_lt (EvClose arg res)) res)
+let lem_theta_close arg res h =
+  assert (thetaP (close arg) h (ev_lt (EvClose arg res)) res) by (compute ())
+
+val destruct_thetaP_open (arg:io_args OOpen) (h:history) (lt:local_trace h) (fs_r:io_res OOpen arg) :
+  Lemma (requires thetaP (openfile arg) h lt fs_r)
+        (ensures (fs_r == Inl (fresh_fd h) /\ lt == [EvOpen arg (Inl (fresh_fd h))]) \/
+                 (fs_r == Inr () /\ lt == [EvOpen arg (Inr ())]))
 let destruct_thetaP_open arg h lt fs_r =
   let p : hist_post h (io_res OOpen arg) = fun lt' r' ->
     (r' == Inl (fresh_fd h) /\ lt' == [EvOpen arg (Inl (fresh_fd h))]) \/
@@ -116,15 +192,9 @@ let destruct_thetaP_open arg h lt fs_r =
     assert (p lt fs_r)
     end
 
-let lem_theta_read arg res h =
-  assert (thetaP (read arg) h (ev_lt (EvRead arg res)) res) by (compute ())
-
-let lem_theta_write arg res h =
-  assert (thetaP (write arg) h (ev_lt (EvWrite arg res)) res) by (compute ())
-
-let lem_theta_close arg res h =
-  assert (thetaP (close arg) h (ev_lt (EvClose arg res)) res) by (compute ())
-
+val destruct_thetaP_read (arg:io_args ORead) (h:history) (lt:local_trace h) (fs_r:io_res ORead arg) :
+  Lemma (requires thetaP (read arg) h lt fs_r)
+        (ensures lt == [EvRead arg fs_r])
 let destruct_thetaP_read arg h lt fs_r =
   let p : hist_post h (io_res ORead arg) = fun lt' r' -> lt' == [EvRead arg r'] in
   match read arg with
@@ -134,6 +204,9 @@ let destruct_thetaP_read arg h lt fs_r =
     assert (p lt fs_r)
     end
 
+val destruct_thetaP_write (arg:io_args OWrite) (h:history) (lt:local_trace h) (fs_r:io_res OWrite arg) :
+  Lemma (requires thetaP (write arg) h lt fs_r)
+        (ensures lt == [EvWrite arg fs_r])
 let destruct_thetaP_write arg h lt fs_r =
   let p : hist_post h (io_res OWrite arg) = fun lt' r' -> lt' == [EvWrite arg r'] in
   match write arg with
@@ -143,6 +216,10 @@ let destruct_thetaP_write arg h lt fs_r =
     assert (p lt fs_r)
     end
 
+
+val destruct_thetaP_close (arg:io_args OClose) (h:history) (lt:local_trace h) (fs_r:io_res OClose arg) :
+  Lemma (requires thetaP (close arg) h lt fs_r)
+        (ensures lt == [EvClose arg fs_r])
 let destruct_thetaP_close arg h lt fs_r =
   let p : hist_post h (io_res OClose arg) = fun lt' r' -> lt' == [EvClose arg r'] in
   match close arg with
@@ -151,6 +228,26 @@ let destruct_thetaP_close arg h lt fs_r =
     assert (theta (close arg) h p) by (compute ());
     assert (p lt fs_r)
     end
+
+let lem_thetaP_return #a (x:a) (h:history) :
+  Lemma (thetaP (return x) h [] x) =
+  theta_monad_morphism_ret x
+
+let lem_thetaP_bind #a #b (m:io a) (h:history) (lt1:local_trace h) (fs_r_m:a) (k:a -> io b) (lt2:local_trace (h++lt1)) (fs_r:b) :
+  Lemma (requires thetaP m h lt1 fs_r_m /\
+                  thetaP (k fs_r_m) (h++lt1) lt2 fs_r)
+        (ensures thetaP (io_bind m k) h (lt1@lt2) fs_r)
+        =
+  wp2p_theta_bind m k;
+  introduce forall (p:hist_post h b). hist_bind (theta m) (fun x -> theta (k x)) h p ==> p (lt1@lt2) fs_r with begin
+    introduce _ ==> _ with _. begin
+      assert (wp2p (theta (k fs_r_m)) (h++lt1) lt2 fs_r);
+      assert (forall (p':hist_post (h++lt1) b). theta (k fs_r_m) (h++lt1) p' ==> p' lt2 fs_r);
+      let p' : hist_post (h++lt1) b = fun lt r -> p (lt1@lt) r in
+      assert (theta (k fs_r_m) (h++lt1) p' ==> p' lt2 fs_r);
+      assert (p (lt1@lt2) fs_r)
+    end
+  end
 
 let thetaP_shift_op_lt #t (o:io_ops) (args:io_args o) (k:io_res o args -> io t) (r:io_res o args) (h:history) (lt:local_trace h)
   : Lemma
@@ -188,7 +285,7 @@ let rec theta_thetaP_in_post #t (m:io t) (h:history) : Lemma (theta m h (fun lt 
           assert (theta (k r) (h ++ lt) (fun lt' fs_r' -> thetaP m h (lt@lt') fs_r'))
         end
       end;
-      assert ((op_wp o args) h (fun lt fs_r -> theta_unf (k fs_r) (h ++ lt) (fun lt' fs_r' -> thetaP m h (lt@lt') fs_r')))
+      assert ((op_wp o args) h (fun lt fs_r -> theta (k fs_r) (h ++ lt) (fun lt' fs_r' -> thetaP m h (lt@lt') fs_r')))
 #pop-options
 
 unfold
@@ -203,7 +300,7 @@ let rec theta_io_bind_exists_ #t1 #t2 (m:io t1) (f:t1 -> io t2) (h:history) : Le
   match m with
   | Return x ->
       theta_thetaP_in_post (f x) h;
-      assert (theta_unf (f x) h (fun lt fs_r -> thetaP (f x) h lt fs_r));
+      assert (theta (f x) h (fun lt fs_r -> thetaP (f x) h lt fs_r));
       calc (hist_post_ord) {
         (fun lt fs_r -> thetaP (f x) h lt fs_r);
         `hist_post_ord` {}
@@ -211,9 +308,9 @@ let rec theta_io_bind_exists_ #t1 #t2 (m:io t1) (f:t1 -> io t2) (h:history) : Le
         `hist_post_ord` {}
         (fun lt fs_r -> exists fs_m lt1 lt2. lt = lt1@lt2 /\ thetaP (Return x) h lt1 fs_m /\ thetaP (f fs_m) (h++lt1) lt2 fs_r);
       };
-      assert (theta_unf (f x) h (theta_io_bind_exists_post m f h))
+      assert (theta (f x) h (theta_io_bind_exists_post m f h))
   | Call o args k ->
-      introduce forall lt r. lt == [op_to_ev o args r] ==> theta_unf (io_bind (k r) f) (h ++ lt) (fun lt' fs_r' -> theta_io_bind_exists_post m f h (lt @ lt') fs_r') with begin
+      introduce forall lt r. lt == [op_to_ev o args r] ==> theta (io_bind (k r) f) (h ++ lt) (fun lt' fs_r' -> theta_io_bind_exists_post m f h (lt @ lt') fs_r') with begin
         introduce _ ==> _ with _. begin
           theta_io_bind_exists_ (k r) f (h ++ lt);
           introduce forall (lt':local_trace (h ++ lt)) fs_r' . theta_io_bind_exists_post (k r) f (h ++ lt) lt' fs_r' ==> theta_io_bind_exists_post m f h (lt @ lt') fs_r' with begin
@@ -236,17 +333,23 @@ let rec theta_io_bind_exists_ #t1 #t2 (m:io t1) (f:t1 -> io t2) (h:history) : Le
               end
             end
           end;
-          assert (theta_unf (io_bind (k r) f) (h ++ lt) (fun lt' r' -> theta_io_bind_exists_post m f h (lt @ lt') r'))
+          assert (theta (io_bind (k r) f) (h ++ lt) (fun lt' r' -> theta_io_bind_exists_post m f h (lt @ lt') r'))
         end
       end;
-      assert (hist_bind (op_wp o args) (fun r -> theta_unf (io_bind (k r) f)) h (theta_io_bind_exists_post m f h));
-      assert (theta_unf (io_bind (Call o args k) f) h (theta_io_bind_exists_post m f h))
+      assert (hist_bind (op_wp o args) (fun r -> theta (io_bind (k r) f)) h (theta_io_bind_exists_post m f h));
+      assert (theta (io_bind (Call o args k) f) h (theta_io_bind_exists_post m f h))
 #pop-options
 
 let theta_io_bind_exists #t1 #t2 (m:io t1) (f:t1 -> io t2) (h:history) : Lemma (theta (io_bind m f) h (theta_io_bind_exists_post m f h)) =
-  unfold_theta #t1 ;
   theta_io_bind_exists_ m f h
 
+val destruct_fs_beh #t1 #t2 (m:io t1) (k:t1 -> io t2) (h:history) (lt:local_trace h) (fs_r:t2) :
+  Lemma
+    (requires thetaP (io_bind m k) h lt fs_r)
+    (ensures exists (lt1:local_trace h) (lt2:local_trace (h++lt1)) (fs_m:t1).
+      lt == (lt1@lt2) /\
+      thetaP m h lt1 fs_m /\
+      thetaP (k fs_m) (h++lt1) lt2 fs_r)
 let destruct_fs_beh #t1 #t2 (m:io t1) (k:t1 -> io t2) (h:history) (lt:local_trace h) (fs_r:t2) :
   Lemma
     (requires thetaP (io_bind m k) h lt fs_r) // forall p. theta (io_bind m k) h p ==> p lt fs_r
